theories/common/CRIS.v
@@ -3,7 +3,7 @@ From iris.proofmode Require Export proofmode.
 
 Require Export FSpec Sp.
 Require Export SMod Mod.
-Require Export ISim ISimFacts WSim ISimNotations WSimNotations.
+Require Export ISim ISimFacts WSim WSimFacts ISimNotations WSimNotations.
 Require Export Tactics TacticsInit IrisTactics.
 
 Require Export CallFilter CtxRefine CtxRefineFacts ClosedAdequacy MainAdequacy.
