theories/simulations/msim/TacticsInit.v
@@ -78,9 +78,3 @@ Ltac init_sim :=
 
 Ltac iinit_simF := initialize_simF.
 
-(* Ltac prove_real_to_img := *)
-(*   iinit_simF; iDestruct "IST" as "->"; iIntros "_"; istep_r; *)
-(*   match goal with |- context[lat_real ?peeking ?fsp] => *)
-(*     iApply (isim_lat_real_to_img peeking fsp) *)
-(*   end; *)
-(*   rewrite !SRed.core !SBRed.choose; refl. *)
